Makes it possible to use several logical steps for one logical steps, in a way which can be controlled by ghost state.

iris/program_logic/total_adequacy.v
@@ -11,15 +11,16 @@ Implicit Types e : expr Λ.
 
 Definition twptp_pre (twptp : list (expr Λ) → iProp Σ)
     (t1 : list (expr Λ)) : iProp Σ :=
-  (∀ t2 σ1 κ κs σ2 n, ⌜step (t1,σ1) κ (t2,σ2)⌝ -∗
-    state_interp σ1 κs n ={⊤}=∗ ∃ n', ⌜κ = []⌝ ∗ state_interp σ2 κs n' ∗ twptp t2)%I.
+  (∀ t2 σ1 ns κ κs σ2 nt, ⌜step (t1,σ1) κ (t2,σ2)⌝ -∗
+    state_interp σ1 ns κs nt ={⊤}=∗
+              ∃ nt', ⌜κ = []⌝ ∗ state_interp σ2 (S ns) κs nt' ∗ twptp t2)%I.
 
 Lemma twptp_pre_mono (twptp1 twptp2 : list (expr Λ) → iProp Σ) :
   ⊢ <pers> (∀ t, twptp1 t -∗ twptp2 t) →
     ∀ t, twptp_pre twptp1 t -∗ twptp_pre twptp2 t.
 Proof.
   iIntros "#H"; iIntros (t) "Hwp". rewrite /twptp_pre.
-  iIntros (t2 σ1 κ κs σ2 n1) "Hstep Hσ".
+  iIntros (t2 σ1 ns κ κs σ2 nt1) "Hstep Hσ".
   iMod ("Hwp" with "[$] [$]") as (n2) "($ & Hσ & ?)".
   iModIntro. iExists n2. iFrame "Hσ". by iApply "H".
 Qed.
@@ -50,7 +51,7 @@ Local Instance twptp_Permutation : Proper ((≡ₚ) ==> (⊢)) twptp.
 Proof.
   iIntros (t1 t1' Ht) "Ht1". iRevert (t1' Ht); iRevert (t1) "Ht1".
   iApply twptp_ind; iIntros "!>" (t1) "IH"; iIntros (t1' Ht).
-  rewrite twptp_unfold /twptp_pre. iIntros (t2 σ1 κ κs σ2 n Hstep) "Hσ".
+  rewrite twptp_unfold /twptp_pre. iIntros (t2 σ1 ns κ κs σ2 nt Hstep) "Hσ".
   destruct (step_Permutation t1' t1 t2 κ σ1 σ2) as (t2'&?&?); [done..|].
   iMod ("IH" $! t2' with "[% //] Hσ") as (n2) "($ & Hσ & IH & _)".
   iModIntro. iExists n2. iFrame "Hσ". by iApply "IH".
@@ -62,7 +63,7 @@ Proof.
   iApply twptp_ind; iIntros "!>" (t1) "IH1". iIntros (t2) "H2".
   iRevert (t1) "IH1"; iRevert (t2) "H2".
   iApply twptp_ind; iIntros "!>" (t2) "IH2". iIntros (t1) "IH1".
-  rewrite twptp_unfold /twptp_pre. iIntros (t1'' σ1 κ κs σ2 n Hstep) "Hσ1".
+  rewrite twptp_unfold /twptp_pre. iIntros (t1'' σ1 ns κ κs σ2 nt Hstep) "Hσ1".
   destruct Hstep as [e1 σ1' e2 σ2' efs' t1' t2' [=Ht ?] ? Hstep]; simplify_eq/=.
   apply app_eq_inv in Ht as [(t&?&?)|(t&?&?)]; subst.
   - destruct t as [|e1' ?]; simplify_eq/=.
@@ -86,27 +87,28 @@ Proof.
   iIntros "He". remember (⊤ : coPset) as E eqn:HE.
   iRevert (HE). iRevert (e E Φ) "He". iApply twp_ind.
   iIntros "!>" (e E Φ); iIntros "IH" (->).
-  rewrite twptp_unfold /twptp_pre /twp_pre. iIntros (t1' σ1' κ κs σ2' n Hstep) "Hσ1".
+  rewrite twptp_unfold /twptp_pre /twp_pre.
+  iIntros (t1' σ1' ns κ κs σ2' nt Hstep) "Hσ1".
   destruct Hstep as [e1 σ1 e2 σ2 efs [|? t1] t2 ?? Hstep];
     simplify_eq/=; try discriminate_list.
   destruct (to_val e1) as [v|] eqn:He1.
   { apply val_stuck in Hstep; naive_solver. }
   iMod ("IH" with "Hσ1") as "[_ IH]".
   iMod ("IH" with "[% //]") as "($ & Hσ & [IH _] & IHfork)".
-  iModIntro. iExists (length efs + n). iFrame "Hσ".
+  iModIntro. iExists (length efs + nt). iFrame "Hσ".
   iApply (twptp_app [_] with "(IH [//])").
   clear. iInduction efs as [|e efs] "IH"; simpl.
-  { rewrite twptp_unfold /twptp_pre. iIntros (t2 σ1 κ κs σ2 n1 Hstep).
+  { rewrite twptp_unfold /twptp_pre. iIntros (t2 σ1 ns κ κs σ2 nt1 Hstep).
     destruct Hstep; simplify_eq/=; discriminate_list. }
   iDestruct "IHfork" as "[[IH' _] IHfork]".
   iApply (twptp_app [_] with "(IH' [//])"). by iApply "IH".
 Qed.
 
-Lemma twptp_total n σ t :
-  state_interp σ [] n -∗ twptp t ={⊤}=∗ ▷ ⌜sn erased_step (t, σ)⌝.
+Lemma twptp_total σ ns nt t :
+  state_interp σ ns [] nt -∗ twptp t ={⊤}=∗ ▷ ⌜sn erased_step (t, σ)⌝.
 Proof.
-  iIntros "Hσ Ht". iRevert (σ n) "Hσ". iRevert (t) "Ht".
-  iApply twptp_ind; iIntros "!>" (t) "IH"; iIntros (σ n) "Hσ".
+  iIntros "Hσ Ht". iRevert (σ ns nt) "Hσ". iRevert (t) "Ht".
+  iApply twptp_ind; iIntros "!>" (t) "IH"; iIntros (σ ns nt) "Hσ".
   iApply (pure_mono _ _ (Acc_intro _)). iIntros ([t' σ'] [κ Hstep]).
   rewrite /twptp_pre.
   iMod ("IH" with "[% //] Hσ") as (n' ->) "[Hσ [H _]]".
@@ -119,13 +121,17 @@ Theorem twp_total Σ Λ `{!invPreG Σ} s e σ Φ :
      ⊢ |={⊤}=> ∃
          (stateI : state Λ → list (observation Λ) → nat → iProp Σ)
          (fork_post : val Λ → iProp Σ),
-       let _ : irisG Λ Σ := IrisG _ _ Hinv stateI fork_post in
+       let _ : irisG Λ Σ :=
+           IrisG _ _ Hinv (λ σ _, stateI σ) fork_post (λ _, 0)
+                 (λ _ _ _ _, fupd_intro _ _)
+       in
        stateI σ [] 0 ∗ WP e @ s; ⊤ [{ Φ }]) →
   sn erased_step ([e], σ). (* i.e. ([e], σ) is strongly normalizing *)
 Proof.
   intros Hwp. apply (soundness (M:=iResUR Σ) _  1); simpl.
   apply (fupd_plain_soundness ⊤ ⊤ _)=> Hinv.
   iMod (Hwp) as (stateI fork_post) "[Hσ H]".
-  iApply (@twptp_total _ _ (IrisG _ _ Hinv stateI fork_post) with "Hσ").
-  by iApply (@twp_twptp _ _ (IrisG _ _ Hinv stateI fork_post)).
+  iApply (@twptp_total _ _ (IrisG _ _ Hinv (λ σ _, stateI σ) fork_post _ _)
+                       _ 0 with "Hσ").
+  by iApply (@twp_twptp _ _ (IrisG _ _ Hinv _ fork_post _ _)).
 Qed.
