iris/program_logic/total_weakestpre.v
@@ -13,12 +13,12 @@ Definition twp_pre `{!irisG Λ Σ} (s : stuckness)
     coPset → expr Λ → (val Λ → iProp Σ) → iProp Σ := λ E e1 Φ,
   match to_val e1 with
   | Some v => |={E}=> Φ v
-  | None => ∀ σ1 κs n,
-     state_interp σ1 κs n ={E,∅}=∗
+  | None => ∀ σ1 ns κs nt,
+     state_interp σ1 ns κs nt ={E,∅}=∗
        ⌜if s is NotStuck then reducible_no_obs e1 σ1 else True⌝ ∗
        ∀ κ e2 σ2 efs, ⌜prim_step e1 σ1 κ e2 σ2 efs⌝ ={∅,E}=∗
          ⌜κ = []⌝ ∗
-         state_interp σ2 κs (length efs + n) ∗
+         state_interp σ2 (S ns) κs (length efs + nt) ∗
          wp E e2 Φ ∗
          [∗ list] ef ∈ efs, wp ⊤ ef fork_post
   end%I.
@@ -32,7 +32,7 @@ Lemma twp_pre_mono `{!irisG Λ Σ} s
 Proof.
   iIntros "#H"; iIntros (E e1 Φ) "Hwp". rewrite /twp_pre.
   destruct (to_val e1) as [v|]; first done.
-  iIntros (σ1 κs n) "Hσ". iMod ("Hwp" with "Hσ") as "($ & Hwp)"; iModIntro.
+  iIntros (σ1 ns κs nt) "Hσ". iMod ("Hwp" with "Hσ") as "($ & Hwp)"; iModIntro.
   iIntros (κ e2 σ2 efs) "Hstep".
   iMod ("Hwp" with "Hstep") as (?) "(Hσ & Hwp & Hfork)".
   iModIntro. iFrame "Hσ". iSplit; first done. iSplitL "Hwp".
@@ -54,7 +54,7 @@ Proof.
     iApply twp_pre_mono. iIntros "!>" (E e Φ). iApply ("H" $! (E,e,Φ)).
   - intros wp Hwp n [[E1 e1] Φ1] [[E2 e2] Φ2]
       [[?%leibniz_equiv ?%leibniz_equiv] ?]; simplify_eq/=.
-    rewrite /uncurry3 /twp_pre. do 24 (f_equiv || done). by apply pair_ne.
+    rewrite /uncurry3 /twp_pre. do 26 (f_equiv || done). by apply pair_ne.
 Qed.
 
 Definition twp_def `{!irisG Λ Σ} : Twp Λ (iProp Σ) stuckness
@@ -115,7 +115,7 @@ Proof.
   iIntros "!>" (e E1 Φ) "IH"; iIntros (E2 Ψ HE) "HΦ".
   rewrite !twp_unfold /twp_pre. destruct (to_val e) as [v|] eqn:?.
   { iApply ("HΦ" with "[> -]"). by iApply (fupd_mask_mono E1 _). }
-  iIntros (σ1 κs n) "Hσ".
+  iIntros (σ1 ns κs nt) "Hσ".
   iMod (fupd_mask_subseteq E1) as "Hclose"; first done.
   iMod ("IH" with "[$]") as "[% IH]".
   iModIntro; iSplit; [by destruct s1, s2|]. iIntros (κ e2 σ2 efs Hstep).
@@ -131,7 +131,7 @@ Lemma fupd_twp s E e Φ : (|={E}=> WP e @ s; E [{ Φ }]) -∗ WP e @ s; E [{ Φ 
 Proof.
   rewrite twp_unfold /twp_pre. iIntros "H". destruct (to_val e) as [v|] eqn:?.
   { by iMod "H". }
-  iIntros (σ1 κs n) "Hσ1". iMod "H". by iApply "H".
+  iIntros (σ1 ns κs nt) "Hσ1". iMod "H". by iApply "H".
 Qed.
 Lemma twp_fupd s E e Φ : WP e @ s; E [{ v, |={E}=> Φ v }] -∗ WP e @ s; E [{ Φ }].
 Proof. iIntros "H". iApply (twp_strong_mono with "H"); auto. Qed.
@@ -142,7 +142,7 @@ Proof.
   iIntros "H". rewrite !twp_unfold /twp_pre /=.
   destruct (to_val e) as [v|] eqn:He.
   { by iDestruct "H" as ">>> $". }
-  iIntros (σ1 κs n) "Hσ". iMod "H". iMod ("H" $! σ1 with "Hσ") as "[$ H]".
+  iIntros (σ1 ns κs nt) "Hσ". iMod "H". iMod ("H" $! σ1 with "Hσ") as "[$ H]".
   iModIntro. iIntros (κ e2 σ2 efs Hstep).
   iMod ("H" with "[//]") as (?) "(Hσ & H & Hefs)". destruct s.
   - rewrite !twp_unfold /twp_pre. destruct (to_val e2) as [v2|] eqn:He2.
@@ -165,7 +165,8 @@ Proof.
   rewrite /twp_pre. destruct (to_val e) as [v|] eqn:He.
   { apply of_to_val in He as <-. iApply fupd_twp. by iApply "HΦ". }
   rewrite twp_unfold /twp_pre fill_not_val //.
-  iIntros (σ1 κs n) "Hσ". iMod ("IH" with "[$]") as "[% IH]". iModIntro; iSplit.
+  iIntros (σ1 ns κs nt) "Hσ". iMod ("IH" with "[$]") as "[% IH]".
+  iModIntro; iSplit.
   { iPureIntro. unfold reducible_no_obs in *.
     destruct s; naive_solver eauto using fill_step. }
   iIntros (κ e2 σ2 efs Hstep).
@@ -186,7 +187,8 @@ Proof.
   { iModIntro. apply of_to_val in He as <-. rewrite !twp_unfold.
     iApply (twp_pre_mono with "[] IH"). by iIntros "!>" (E e Φ') "[_ ?]". }
   rewrite /twp_pre fill_not_val //.
-  iIntros (σ1 κs n) "Hσ". iMod ("IH" with "[$]") as "[% IH]". iModIntro; iSplit.
+  iIntros (σ1 ns κs nt) "Hσ". iMod ("IH" with "[$]") as "[% IH]".
+  iModIntro; iSplit.
   { destruct s; eauto using reducible_no_obs_fill_inv. }
   iIntros (κ e2 σ2 efs Hstep).
   iMod ("IH" $! κ (K e2) σ2 efs with "[]") as (?) "(Hσ & IH & IHefs)"; eauto using fill_step.
@@ -198,12 +200,14 @@ Qed.
 Lemma twp_wp s E e Φ : WP e @ s; E [{ Φ }] -∗ WP e @ s; E {{ Φ }}.
 Proof.
   iIntros "H". iLöb as "IH" forall (E e Φ).
-  rewrite wp_unfold twp_unfold /wp_pre /twp_pre. destruct (to_val e) as [v|]=>//.
-  iIntros (σ1 κ κs n) "Hσ". iMod ("H" with "Hσ") as "[% H]". iIntros "!>". iSplitR.
+  rewrite wp_unfold twp_unfold /wp_pre /twp_pre. destruct (to_val e) as [v|]=>//=.
+  iIntros (σ1 ns κ κs nt) "Hσ". iMod ("H" with "Hσ") as "[% H]".
+  iIntros "!>". iSplitR.
   { destruct s; eauto using reducible_no_obs_reducible. }
   iIntros (e2 σ2 efs) "Hstep". iMod ("H" with "Hstep") as (->) "(Hσ & H & Hfork)".
-  iApply step_fupd_intro; [set_solver+|]. iNext.
-  iFrame "Hσ". iSplitL "H".
+  iApply fupd_mask_intro; [set_solver+|]. iIntros "Hclose".
+  iIntros "!>!>". iApply step_fupdN_intro=>//. iModIntro. iMod "Hclose" as "_".
+  iModIntro. iFrame "Hσ". iSplitL "H".
   { by iApply "IH". }
   iApply (@big_sepL_impl with "Hfork").
   iIntros "!>" (k ef _) "H". by iApply "IH".
