iris/program_logic/weakestpre.v
@@ -10,17 +10,40 @@ Import uPred.
 Class irisG (Λ : language) (Σ : gFunctors) := IrisG {
   iris_invG :> invG Σ;
 
-  (** The state interpretation is an invariant that should hold in between each
-  step of reduction. Here [Λstate] is the global state, [list Λobservation] are
-  the remaining observations, and [nat] is the number of forked-off threads
-  (not the total number of threads, which is one higher because there is always
-  a main thread). *)
-  state_interp : state Λ → list (observation Λ) → nat → iProp Σ;
+  (** The state interpretation is an invariant that should hold in
+  between each step of reduction. Here [Λstate] is the global state,
+  the first [nat] is the number of steps already performed by the
+  program, [list Λobservation] are the remaining observations, and the
+  last [nat] is the number of forked-off threads (not the total number
+  of threads, which is one higher because there is always a main
+  thread). *)
+  state_interp : state Λ → nat → list (observation Λ) → nat → iProp Σ;
 
   (** A fixed postcondition for any forked-off thread. For most languages, e.g.
   heap_lang, this will simply be [True]. However, it is useful if one wants to
   keep track of resources precisely, as in e.g. Iron. *)
   fork_post : val Λ → iProp Σ;
+
+  (** Number of additional logical steps (i.e., later modality in the
+  definition of WP) per physical step, depending on the physical steps
+  counter. In addition to these steps, the definition of WP adds one
+  extra later per physical step to make sure that there is at least
+  one later for each physical step. *)
+  num_laters_per_step : nat → nat;
+
+  (** When performing pure steps, the state interpretation needs to be
+  adapted for the change in the [ns] parameter.
+
+  Note that we use an empty-mask fancy update here. We could also use
+  a basic update or a bare magic wand, the expressiveness of the
+  framework would be the same. If we removed the modality here, then
+  the client would have to include the modality it needs as part of
+  the definition of [state_interp]. Since adding the modality as part
+  of the definition [state_interp_mono] does not significantly
+  complicate the formalization in Iris, we prefer simplifying the
+  client. *)
+  state_interp_mono σ ns κs nt:
+    state_interp σ ns κs nt ={∅}=∗ state_interp σ (S ns) κs nt
 }.
 Global Opaque iris_invG.
 
@@ -29,19 +52,25 @@ Definition wp_pre `{!irisG Λ Σ} (s : stuckness)
     coPset -d> expr Λ -d> (val Λ -d> iPropO Σ) -d> iPropO Σ := λ E e1 Φ,
   match to_val e1 with
   | Some v => |={E}=> Φ v
-  | None => ∀ σ1 κ κs n,
-     state_interp σ1 (κ ++ κs) n ={E,∅}=∗
+  | None => ∀ σ1 ns κ κs nt,
+     state_interp σ1 ns (κ ++ κs) nt ={E,∅}=∗
        ⌜if s is NotStuck then reducible e1 σ1 else True⌝ ∗
-       ∀ e2 σ2 efs, ⌜prim_step e1 σ1 κ e2 σ2 efs⌝ ={∅}=∗ ▷ |={∅,E}=>
-         state_interp σ2 κs (length efs + n) ∗
+       ∀ e2 σ2 efs, ⌜prim_step e1 σ1 κ e2 σ2 efs⌝
+         ={∅}▷=∗^(S $ num_laters_per_step ns) |={∅,E}=>
+         state_interp σ2 (S ns) κs (length efs + nt) ∗
          wp E e2 Φ ∗
          [∗ list] i ↦ ef ∈ efs, wp ⊤ ef fork_post
   end%I.
 
 Local Instance wp_pre_contractive `{!irisG Λ Σ} s : Contractive (wp_pre s).
 Proof.
-  rewrite /wp_pre=> n wp wp' Hwp E e1 Φ.
-  repeat (f_contractive || f_equiv); apply Hwp.
+  rewrite /wp_pre /= => n wp wp' Hwp E e1 Φ.
+  do 24 (f_contractive || f_equiv).
+  (* FIXME : simplify this proof once we have a good definition and a
+     proper instance for step_fupdN. *)
+  induction num_laters_per_step as [|k IH]; simpl.
+  - repeat (f_contractive || f_equiv); apply Hwp.
+  - by rewrite -IH.
 Qed.
 
 Definition wp_def `{!irisG Λ Σ} : Wp Λ (iProp Σ) stuckness :=
@@ -70,12 +99,15 @@ Global Instance wp_ne s E e n :
   Proper (pointwise_relation _ (dist n) ==> dist n) (wp (PROP:=iProp Σ) s E e).
 Proof.
   revert e. induction (lt_wf n) as [n _ IH]=> e Φ Ψ HΦ.
-  rewrite !wp_unfold /wp_pre.
+  rewrite !wp_unfold /wp_pre /=.
   (* FIXME: figure out a way to properly automate this proof *)
   (* FIXME: reflexivity, as being called many times by f_equiv and f_contractive
   is very slow here *)
-  do 24 (f_contractive || f_equiv). apply IH; first lia.
-  intros v. eapply dist_le; eauto with lia.
+  do 24 (f_contractive || f_equiv).
+  (* FIXME : simplify this proof once we have a good definition and a
+     proper instance for step_fupdN. *)
+  induction num_laters_per_step as [|k IHk]; simpl; last by rewrite IHk.
+  rewrite IH; [done|lia|]. intros v. eapply dist_S, HΦ.
 Qed.
 Global Instance wp_proper s E e :
   Proper (pointwise_relation _ (≡) ==> (≡)) (wp (PROP:=iProp Σ) s E e).
@@ -86,8 +118,12 @@ Global Instance wp_contractive s E e n :
   TCEq (to_val e) None →
   Proper (pointwise_relation _ (dist_later n) ==> dist n) (wp (PROP:=iProp Σ) s E e).
 Proof.
-  intros He Φ Ψ HΦ. rewrite !wp_unfold /wp_pre He.
-  by repeat (f_contractive || f_equiv).
+  intros He Φ Ψ HΦ. rewrite !wp_unfold /wp_pre He /=.
+  do 23 (f_contractive || f_equiv).
+  (* FIXME : simplify this proof once we have a good definition and a
+     proper instance for step_fupdN. *)
+  induction num_laters_per_step as [|k IHk]; simpl; last by rewrite IHk.
+  by do 4 f_equiv.
 Qed.
 
 Lemma wp_value_fupd' s E Φ v : WP of_val v @ s; E {{ Φ }} ⊣⊢ |={E}=> Φ v.
@@ -98,16 +134,16 @@ Lemma wp_strong_mono s1 s2 E1 E2 e Φ Ψ :
   WP e @ s1; E1 {{ Φ }} -∗ (∀ v, Φ v ={E2}=∗ Ψ v) -∗ WP e @ s2; E2 {{ Ψ }}.
 Proof.
   iIntros (? HE) "H HΦ". iLöb as "IH" forall (e E1 E2 HE Φ Ψ).
-  rewrite !wp_unfold /wp_pre.
+  rewrite !wp_unfold /wp_pre /=.
   destruct (to_val e) as [v|] eqn:?.
   { iApply ("HΦ" with "[> -]"). by iApply (fupd_mask_mono E1 _). }
-  iIntros (σ1 κ κs n) "Hσ".
+  iIntros (σ1 ns κ κs nt) "Hσ".
   iMod (fupd_mask_subseteq E1) as "Hclose"; first done.
   iMod ("H" with "[$]") as "[% H]".
   iModIntro. iSplit; [by destruct s1, s2|]. iIntros (e2 σ2 efs Hstep).
-  iMod ("H" with "[//]") as "H". iIntros "!> !>".
-  iMod "H" as "(Hσ & H & Hefs)".
-  iMod "Hclose" as "_". iModIntro. iFrame "Hσ". iSplitR "Hefs".
+  iMod ("H" with "[//]") as "H". iIntros "!> !>".  iMod "H". iModIntro.
+  iApply (step_fupdN_wand with "[H]"); first by iApply "H".
+  iIntros ">($ & H & Hefs)". iMod "Hclose" as "_". iModIntro. iSplitR "Hefs".
   - iApply ("IH" with "[//] H HΦ").
   - iApply (big_sepL_impl with "Hefs"); iIntros "!>" (k ef _).
     iIntros "H". iApply ("IH" with "[] H"); auto.
@@ -117,7 +153,7 @@ Lemma fupd_wp s E e Φ : (|={E}=> WP e @ s; E {{ Φ }}) ⊢ WP e @ s; E {{ Φ }}
 Proof.
   rewrite wp_unfold /wp_pre. iIntros "H". destruct (to_val e) as [v|] eqn:?.
   { by iMod "H". }
-  iIntros (σ1 κ κs n) "Hσ1". iMod "H". by iApply "H".
+  iIntros (σ1 ns κ κs nt) "Hσ1". iMod "H". by iApply "H".
 Qed.
 Lemma wp_fupd s E e Φ : WP e @ s; E {{ v, |={E}=> Φ v }} ⊢ WP e @ s; E {{ Φ }}.
 Proof. iIntros "H". iApply (wp_strong_mono s s E with "H"); auto. Qed.
@@ -128,30 +164,54 @@ Proof.
   iIntros "H". rewrite !wp_unfold /wp_pre.
   destruct (to_val e) as [v|] eqn:He.
   { by iDestruct "H" as ">>> $". }
-  iIntros (σ1 κ κs n) "Hσ". iMod "H". iMod ("H" $! σ1 with "Hσ") as "[$ H]".
+  iIntros (σ1 ns κ κs nt) "Hσ". iMod "H". iMod ("H" $! σ1 with "Hσ") as "[$ H]".
   iModIntro. iIntros (e2 σ2 efs Hstep).
-  iMod ("H" with "[//]") as "H". iIntros "!>!>".
-  iMod "H" as "(Hσ & H & Hefs)". destruct s.
+  iApply (step_fupdN_wand with "[H]"); first by iApply "H".
+  iIntros ">(Hσ & H & Hefs)". destruct s.
   - rewrite !wp_unfold /wp_pre. destruct (to_val e2) as [v2|] eqn:He2.
     + iDestruct "H" as ">> $". by iFrame.
-    + iMod ("H" $! _ [] with "[$]") as "[H _]". iDestruct "H" as %(? & ? & ? & ? & ?).
+    + iMod ("H" $! _ _ [] with "[$]") as "[H _]". iDestruct "H" as %(? & ? & ? & ? & ?).
       by edestruct (atomic _ _ _ _ _ Hstep).
   - destruct (atomic _ _ _ _ _ Hstep) as [v <-%of_to_val].
     rewrite wp_value_fupd'. iMod "H" as ">H".
     iModIntro. iFrame "Hσ Hefs". by iApply wp_value_fupd'.
 Qed.
 
-Lemma wp_step_fupd s E1 E2 e P Φ :
+(** In this stronger version of [wp_step_fupdN], the masks in the
+   step-taking fancy update are a bit weird and somewhat difficult to
+   use in practice. Hence, we prove it for the sake of completeness,
+   but [wp_step_fupdN] is just a little bit weaker, suffices in
+   practice and is easier to use.
+
+   See the statement of [wp_step_fupdN] below to understand the use of
+   ordinary conjunction here. *)
+Lemma wp_step_fupdN_strong n s E1 E2 e P Φ :
   TCEq (to_val e) None → E2 ⊆ E1 →
-  (|={E1}[E2]▷=> P) -∗ WP e @ s; E2 {{ v, P ={E1}=∗ Φ v }} -∗ WP e @ s; E1 {{ Φ }}.
+  (∀ σ ns κs nt, state_interp σ ns κs nt
+       ={E1,∅}=∗ ⌜n ≤ S (num_laters_per_step ns)⌝) ∧
+  ((|={E1,E2}=> |={∅}▷=>^n |={E2,E1}=> P) ∗
+    WP e @ s; E2 {{ v, P ={E1}=∗ Φ v }}) -∗
+  WP e @ s; E1 {{ Φ }}.
 Proof.
-  rewrite !wp_unfold /wp_pre. iIntros (-> ?) "HR H".
-  iIntros (σ1 κ κs n) "Hσ". iMod "HR". iMod ("H" with "[$]") as "[$ H]".
+  destruct n as [|n].
+  { iIntros (_ ?) "/= [_ [HP Hwp]]".
+    iApply (wp_strong_mono with "Hwp"); [done..|].
+    iIntros (v) "H". iApply ("H" with "[>HP]"). by do 2 iMod "HP". }
+  rewrite !wp_unfold /wp_pre /=. iIntros (-> ?) "H".
+  iIntros (σ1 ns κ κs nt) "Hσ".
+  destruct (decide (n ≤ num_laters_per_step ns)) as [Hn|Hn]; first last.
+  { iDestruct "H" as "[Hn _]". iMod ("Hn" with "Hσ") as %?. lia. }
+  iDestruct "H" as "[_ [>HP Hwp]]". iMod ("Hwp" with "[$]") as "[$ H]". iMod "HP".
   iIntros "!>" (e2 σ2 efs Hstep). iMod ("H" $! e2 σ2 efs with "[% //]") as "H".
-  iIntros "!>!>". iMod "H" as "(Hσ & H & Hefs)".
-  iMod "HR". iModIntro. iFrame "Hσ Hefs".
-  iApply (wp_strong_mono s s E2 with "H"); [done..|].
-  iIntros (v) "H". by iApply "H".
+  iIntros "!>!>". iMod "H". iMod "HP". iModIntro.
+  revert n Hn. generalize (num_laters_per_step ns)=>n0 n Hn.
+  iInduction n as [|n] "IH" forall (n0 Hn).
+  - iApply (step_fupdN_wand with "H"). iIntros ">($ & Hwp & $)". iMod "HP".
+    iModIntro. iApply (wp_strong_mono with "Hwp"); [done|set_solver|].
+    iIntros (v) "HΦ". iApply ("HΦ" with "HP").
+  - destruct n0 as [|n0]; [lia|]=>/=. iMod "HP". iMod "H". iIntros "!> !>".
+    iMod "HP". iMod "H". iModIntro. iApply ("IH" with "[] HP H").
+    auto with lia.
 Qed.
 
 Lemma wp_bind K `{!LanguageCtx K} s E e Φ :
@@ -160,29 +220,31 @@ Proof.
   iIntros "H". iLöb as "IH" forall (E e Φ). rewrite wp_unfold /wp_pre.
   destruct (to_val e) as [v|] eqn:He.
   { apply of_to_val in He as <-. by iApply fupd_wp. }
-  rewrite wp_unfold /wp_pre fill_not_val //.
-  iIntros (σ1 κ κs n) "Hσ". iMod ("H" with "[$]") as "[% H]". iModIntro; iSplit.
+  rewrite wp_unfold /wp_pre fill_not_val /=; [|done].
+  iIntros (σ1 step κ κs n) "Hσ". iMod ("H" with "[$]") as "[% H]".
+  iModIntro; iSplit.
   { destruct s; eauto using reducible_fill. }
   iIntros (e2 σ2 efs Hstep).
   destruct (fill_step_inv e σ1 κ e2 σ2 efs) as (e2'&->&?); auto.
   iMod ("H" $! e2' σ2 efs with "[//]") as "H". iIntros "!>!>".
-  iMod "H" as "(Hσ & H & Hefs)".
-  iModIntro. iFrame "Hσ Hefs". by iApply "IH".
+  iMod "H". iModIntro. iApply (step_fupdN_wand with "H"). iIntros "H".
+  iMod "H" as "($ & H & $)". iModIntro. by iApply "IH".
 Qed.
 
 Lemma wp_bind_inv K `{!LanguageCtx K} s E e Φ :
   WP K e @ s; E {{ Φ }} ⊢ WP e @ s; E {{ v, WP K (of_val v) @ s; E {{ Φ }} }}.
 Proof.
-  iIntros "H". iLöb as "IH" forall (E e Φ). rewrite !wp_unfold /wp_pre.
+  iIntros "H". iLöb as "IH" forall (E e Φ). rewrite !wp_unfold /wp_pre /=.
   destruct (to_val e) as [v|] eqn:He.
   { apply of_to_val in He as <-. by rewrite !wp_unfold /wp_pre. }
   rewrite fill_not_val //.
-  iIntros (σ1 κ κs n) "Hσ". iMod ("H" with "[$]") as "[% H]". iModIntro; iSplit.
+  iIntros (σ1 ns κ κs nt) "Hσ". iMod ("H" with "[$]") as "[% H]".
+  iModIntro; iSplit.
   { destruct s; eauto using reducible_fill_inv. }
   iIntros (e2 σ2 efs Hstep).
-  iMod ("H" $! (K e2) σ2 efs with "[]") as "H"; [by eauto using fill_step|].
-  iIntros "!>!>". iMod "H" as "(Hσ & H & Hefs)".
-  iModIntro. iFrame "Hσ Hefs". by iApply "IH".
+  iMod ("H" $! _ _ _ with "[]") as "H"; first eauto using fill_step.
+  iIntros "!> !>". iMod "H". iModIntro. iApply (step_fupdN_wand with "H").
+  iIntros "H". iMod "H" as "($ & H & $)". iModIntro. by iApply "IH".
 Qed.
 
 (** * Derived rules *)
@@ -217,6 +279,41 @@ Lemma wp_frame_l s E e Φ R : R ∗ WP e @ s; E {{ Φ }} ⊢ WP e @ s; E {{ v, R
 Proof. iIntros "[? H]". iApply (wp_strong_mono with "H"); auto with iFrame. Qed.
 Lemma wp_frame_r s E e Φ R : WP e @ s; E {{ Φ }} ∗ R ⊢ WP e @ s; E {{ v, Φ v ∗ R }}.
 Proof. iIntros "[H ?]". iApply (wp_strong_mono with "H"); auto with iFrame. Qed.
+
+(** This lemma states that if we can prove that [n] laters are used in
+   the current physical step, then one can perform an n-steps fancy
+   update during that physical step. The resources needed to prove the
+   bound on [n] are not used up: they can be reused in the proof of
+   the WP or in the proof of the n-steps fancy update. In order to
+   describe this unusual resource flow, we use ordinary conjunction as
+   a premise. *)
+Lemma wp_step_fupdN n s E1 E2 e P Φ :
+  TCEq (to_val e) None → E2 ⊆ E1 →
+  (∀ σ ns κs nt, state_interp σ ns κs nt
+       ={E1,∅}=∗ ⌜n ≤ S (num_laters_per_step ns)⌝) ∧
+  ((|={E1∖E2,∅}=> |={∅}▷=>^n |={∅,E1∖E2}=> P) ∗
+    WP e @ s; E2 {{ v, P ={E1}=∗ Φ v }}) -∗
+  WP e @ s; E1 {{ Φ }}.
+Proof.
+  iIntros (??) "H". iApply (wp_step_fupdN_strong with "[H]"); [done|].
+  iApply (and_mono_r with "H"). apply sep_mono_l. iIntros "HP".
+  iMod fupd_mask_subseteq_emptyset_difference as "H"; [|iMod "HP"]; [set_solver|].
+  iMod "H" as "_". replace (E1 ∖ (E1 ∖ E2)) with E2; last first.
+  { set_unfold=>x. destruct (decide (x ∈ E2)); naive_solver. }
+  iModIntro. iApply (step_fupdN_wand with "HP"). iIntros "H".
+  iApply fupd_mask_frame; [|iMod "H"; iModIntro]; [set_solver|].
+  by rewrite difference_empty_L (comm_L (∪)) -union_difference_L.
+Qed.
+Lemma wp_step_fupd s E1 E2 e P Φ :
+  TCEq (to_val e) None → E2 ⊆ E1 →
+  (|={E1}[E2]▷=> P) -∗ WP e @ s; E2 {{ v, P ={E1}=∗ Φ v }} -∗ WP e @ s; E1 {{ Φ }}.
+Proof.
+  iIntros (??) "HR H".
+  iApply (wp_step_fupdN_strong 1 _ E1 E2 with "[-]"); [done|..]. iSplit.
+  - iIntros (????) "_". iMod (fupd_mask_subseteq ∅) as "_"; [set_solver+|].
+    auto with lia.
+  - iFrame "H". iMod "HR" as "$". auto.
+Qed.
 
 Lemma wp_frame_step_l s E1 E2 e Φ R :
   TCEq (to_val e) None → E2 ⊆ E1 →
@@ -257,7 +354,6 @@ Proof.
   iIntros "[HQ HWP]". iApply (wp_wand with "HWP").
   iIntros (v) "HΦ". by iApply "HΦ".
 Qed.
-
 End wp.
 
 (** Proofmode class instances *)
