iris/program_logic/ectx_lifting.v
@@ -17,15 +17,15 @@ Local Hint Resolve head_stuck_stuck : core.
 
 Lemma wp_lift_head_step_fupd {s E Φ} e1 :
   to_val e1 = None →
-  (∀ σ1 κ κs n, state_interp σ1 (κ ++ κs) n ={E,∅}=∗
+  (∀ σ1 ns κ κs nt, state_interp σ1 ns (κ ++ κs) nt ={E,∅}=∗
     ⌜head_reducible e1 σ1⌝ ∗
     ∀ e2 σ2 efs, ⌜head_step e1 σ1 κ e2 σ2 efs⌝ ={∅}=∗ ▷ |={∅,E}=>
-      state_interp σ2 κs (length efs + n) ∗
+      state_interp σ2 (S ns) κs (length efs + nt) ∗
       WP e2 @ s; E {{ Φ }} ∗
       [∗ list] ef ∈ efs, WP ef @ s; ⊤ {{ fork_post }})
   ⊢ WP e1 @ s; E {{ Φ }}.
 Proof.
-  iIntros (?) "H". iApply wp_lift_step_fupd=>//. iIntros (σ1 κ κs Qs) "Hσ".
+  iIntros (?) "H". iApply wp_lift_step_fupd=>//. iIntros (σ1 ns κ κs nt) "Hσ".
   iMod ("H" with "Hσ") as "[% H]"; iModIntro.
   iSplit; first by destruct s; eauto. iIntros (e2 σ2 efs ?).
   iApply "H"; eauto.
@@ -33,26 +33,26 @@ Qed.
 
 Lemma wp_lift_head_step {s E Φ} e1 :
   to_val e1 = None →
-  (∀ σ1 κ κs n, state_interp σ1 (κ ++ κs) n ={E,∅}=∗
+  (∀ σ1 ns κ κs nt, state_interp σ1 ns (κ ++ κs) nt ={E,∅}=∗
     ⌜head_reducible e1 σ1⌝ ∗
     ▷ ∀ e2 σ2 efs, ⌜head_step e1 σ1 κ e2 σ2 efs⌝ ={∅,E}=∗
-      state_interp σ2 κs (length efs + n) ∗
+      state_interp σ2 (S ns) κs (length efs + nt) ∗
       WP e2 @ s; E {{ Φ }} ∗
       [∗ list] ef ∈ efs, WP ef @ s; ⊤ {{ fork_post }})
   ⊢ WP e1 @ s; E {{ Φ }}.
 Proof.
-  iIntros (?) "H". iApply wp_lift_head_step_fupd; [done|]. iIntros (????) "?".
+  iIntros (?) "H". iApply wp_lift_head_step_fupd; [done|]. iIntros (?????) "?".
   iMod ("H" with "[$]") as "[$ H]". iIntros "!>" (e2 σ2 efs ?) "!> !>". by iApply "H".
 Qed.
 
 Lemma wp_lift_head_stuck E Φ e :
   to_val e = None →
   sub_redexes_are_values e →
-  (∀ σ κs n, state_interp σ κs n ={E,∅}=∗ ⌜head_stuck e σ⌝)
+  (∀ σ ns κs nt, state_interp σ ns κs nt ={E,∅}=∗ ⌜head_stuck e σ⌝)
   ⊢ WP e @ E ?{{ Φ }}.
 Proof.
   iIntros (??) "H". iApply wp_lift_stuck; first done.
-  iIntros (σ κs n) "Hσ". iMod ("H" with "Hσ") as "%". by auto.
+  iIntros (σ ns κs nt) "Hσ". iMod ("H" with "Hσ") as "%". by auto.
 Qed.
 
 Lemma wp_lift_pure_head_stuck E Φ e :
@@ -62,51 +62,51 @@ Lemma wp_lift_pure_head_stuck E Φ e :
   ⊢ WP e @ E ?{{ Φ }}.
 Proof using Hinh.
   iIntros (?? Hstuck). iApply wp_lift_head_stuck; [done|done|].
-  iIntros (σ κs n) "_". iApply fupd_mask_intro; by auto with set_solver.
+  iIntros (σ ns κs nt) "_". iApply fupd_mask_intro; by auto with set_solver.
 Qed.
 
 Lemma wp_lift_atomic_head_step_fupd {s E1 E2 Φ} e1 :
   to_val e1 = None →
-  (∀ σ1 κ κs n, state_interp σ1 (κ ++ κs) n ={E1}=∗
+  (∀ σ1 ns κ κs nt, state_interp σ1 ns (κ ++ κs) nt ={E1}=∗
     ⌜head_reducible e1 σ1⌝ ∗
     ∀ e2 σ2 efs, ⌜head_step e1 σ1 κ e2 σ2 efs⌝ ={E1}[E2]▷=∗
-      state_interp σ2 κs (length efs + n) ∗
+      state_interp σ2 (S ns) κs (length efs + nt) ∗
       from_option Φ False (to_val e2) ∗
       [∗ list] ef ∈ efs, WP ef @ s; ⊤ {{ fork_post }})
   ⊢ WP e1 @ s; E1 {{ Φ }}.
 Proof.
   iIntros (?) "H". iApply wp_lift_atomic_step_fupd; [done|].
-  iIntros (σ1 κ κs Qs) "Hσ1". iMod ("H" with "Hσ1") as "[% H]"; iModIntro.
+  iIntros (σ1 ns κ κs nt) "Hσ1". iMod ("H" with "Hσ1") as "[% H]"; iModIntro.
   iSplit; first by destruct s; auto. iIntros (e2 σ2 efs Hstep).
   iApply "H"; eauto.
 Qed.
 
 Lemma wp_lift_atomic_head_step {s E Φ} e1 :
   to_val e1 = None →
-  (∀ σ1 κ κs n, state_interp σ1 (κ ++ κs) n ={E}=∗
+  (∀ σ1 ns κ κs nt, state_interp σ1 ns (κ ++ κs) nt ={E}=∗
     ⌜head_reducible e1 σ1⌝ ∗
     ▷ ∀ e2 σ2 efs, ⌜head_step e1 σ1 κ e2 σ2 efs⌝ ={E}=∗
-      state_interp σ2 κs (length efs + n) ∗
+      state_interp σ2 (S ns) κs (length efs + nt) ∗
       from_option Φ False (to_val e2) ∗
       [∗ list] ef ∈ efs, WP ef @ s; ⊤ {{ fork_post }})
   ⊢ WP e1 @ s; E {{ Φ }}.
 Proof.
   iIntros (?) "H". iApply wp_lift_atomic_step; eauto.
-  iIntros (σ1 κ κs Qs) "Hσ1". iMod ("H" with "Hσ1") as "[% H]"; iModIntro.
+  iIntros (σ1 ns κ κs nt) "Hσ1". iMod ("H" with "Hσ1") as "[% H]"; iModIntro.
   iSplit; first by destruct s; auto. iNext. iIntros (e2 σ2 efs Hstep).
   iApply "H"; eauto.
 Qed.
 
 Lemma wp_lift_atomic_head_step_no_fork_fupd {s E1 E2 Φ} e1 :
   to_val e1 = None →
-  (∀ σ1 κ κs n, state_interp σ1 (κ ++ κs) n ={E1}=∗
+  (∀ σ1 ns κ κs nt, state_interp σ1 ns (κ ++ κs) nt ={E1}=∗
     ⌜head_reducible e1 σ1⌝ ∗
     ∀ e2 σ2 efs, ⌜head_step e1 σ1 κ e2 σ2 efs⌝ ={E1}[E2]▷=∗
-      ⌜efs = []⌝ ∗ state_interp σ2 κs n ∗ from_option Φ False (to_val e2))
+      ⌜efs = []⌝ ∗ state_interp σ2 (S ns) κs nt ∗ from_option Φ False (to_val e2))
   ⊢ WP e1 @ s; E1 {{ Φ }}.
 Proof.
   iIntros (?) "H". iApply wp_lift_atomic_head_step_fupd; [done|].
-  iIntros (σ1 κ κs Qs) "Hσ1". iMod ("H" $! σ1 with "Hσ1") as "[$ H]"; iModIntro.
+  iIntros (σ1 ns κ κs nt) "Hσ1". iMod ("H" $! σ1 with "Hσ1") as "[$ H]"; iModIntro.
   iIntros (v2 σ2 efs Hstep).
   iMod ("H" $! v2 σ2 efs with "[# //]") as "H".
   iIntros "!> !>". iMod "H" as "(-> & ? & ?) /=". by iFrame.
@@ -114,14 +114,14 @@ Qed.
 
 Lemma wp_lift_atomic_head_step_no_fork {s E Φ} e1 :
   to_val e1 = None →
-  (∀ σ1 κ κs n, state_interp σ1 (κ ++ κs) n ={E}=∗
+  (∀ σ1 ns κ κs nt, state_interp σ1 ns (κ ++ κs) nt ={E}=∗
     ⌜head_reducible e1 σ1⌝ ∗
     ▷ ∀ e2 σ2 efs, ⌜head_step e1 σ1 κ e2 σ2 efs⌝ ={E}=∗
-      ⌜efs = []⌝ ∗ state_interp σ2 κs n ∗ from_option Φ False (to_val e2))
+      ⌜efs = []⌝ ∗ state_interp σ2 (S ns) κs nt ∗ from_option Φ False (to_val e2))
   ⊢ WP e1 @ s; E {{ Φ }}.
 Proof.
   iIntros (?) "H". iApply wp_lift_atomic_head_step; eauto.
-  iIntros (σ1 κ κs Qs) "Hσ1". iMod ("H" $! σ1 with "Hσ1") as "[$ H]"; iModIntro.
+  iIntros (σ1 ns κ κs nt) "Hσ1". iMod ("H" $! σ1 with "Hσ1") as "[$ H]"; iModIntro.
   iNext; iIntros (v2 σ2 efs Hstep).
   iMod ("H" $! v2 σ2 efs with "[//]") as "(-> & ? & ?) /=". by iFrame.
 Qed.
